WIP, start defining comparison

Ordinal/Notation/BHTowerNotation.v
@@ -50,8 +50,17 @@ Local Hint Resolve
 
 Inductive BHForm := BH : list BHForm -> BHForm.
 
-Fixpoint BH_denote (v:BHForm) : Ord :=
-  match v with
+Fixpoint BH_termSize (x:BHForm) : nat :=
+  match x with
+  | BH l => 1%nat + fold_right Nat.add 0%nat (map BH_termSize l)
+  end.
+
+Definition BH_listSize (xs:list BHForm) : nat :=
+  fold_right Nat.add 0%nat (map BH_termSize xs).
+
+
+Fixpoint BH_denote (x:BHForm) : Ord :=
+  match x with
   | BH l => BH_full_stack (map BH_denote l)
   end.
 
@@ -180,3 +189,413 @@ Proof.
   apply BH2_correct.
   apply BH2_correct.
 Qed.
+
+
+Definition bh_isZero (x:BHForm) : bool :=
+  match x with
+  | BH [] => true
+  | _     => false
+  end.
+
+Fixpoint bh_allZero (xs: list BHForm) : bool :=
+  match xs with
+  | [] => true
+  | (x::xs) => if bh_isZero x then bh_allZero xs else false
+  end.
+
+Definition isNil (xs:list BHForm) : bool :=
+  match xs with
+  | [] => true
+  | _  => false
+  end.
+
+Reserved Notation "{ x , y } ~~~> z" (at level 70, format "{ x , y }  ~~~>  z"). 
+Reserved Notation "{ a , x , y , b } ~~> z" (at level 70, format "{ a , x , y , b }  ~~>  z"). 
+
+Inductive BH_compare_graph : BHForm -> BHForm -> ordering -> Prop :=
+
+| BH_compare_node : forall xs ys o,
+    { BH xs, xs, ys, BH ys } ~~> o  ->
+    { BH xs, BH ys } ~~~> o
+
+where "{ x , y } ~~~> z" := (BH_compare_graph x y z)
+
+with BH_compare_seq_graph : BHForm -> list BHForm -> list BHForm -> BHForm -> ordering -> Prop :=
+| BH_compare_zero_eq: forall xtop ytop,
+    { xtop, [], [], ytop } ~~> EQ
+
+| BH_compare_zero_l: forall xtop ytop y ys,
+    { xtop, [], (y::ys), ytop } ~~> LT
+
+| BH_compare_zero_r: forall xtop ytop x xs,
+    { xtop, (x::xs), [], ytop } ~~> GT
+
+| BH_compare_one: forall xtop ytop x y o,
+    { x, y } ~~~> o ->
+    { xtop, [x], [y], ytop } ~~> o
+
+| BH_compare_leading_zero_l : forall xtop ytop x xs ys o,
+    x = BH [] ->
+    xs <> [] ->
+    { xtop, xs, ys, ytop } ~~> o ->
+    { xtop, x::xs, ys, ytop } ~~> o
+
+| BH_compare_leading_zero_r : forall xtop ytop xs y ys o,
+    y = BH [] ->
+    ys <> [] ->
+    { xtop, xs, ys, ytop } ~~> o ->
+    { xtop, xs, y::ys, ytop } ~~> o
+
+| BH_compare_head_eq : forall xtop ytop x xs y ys o,
+    length xs = length ys ->
+    { x, y } ~~~> EQ ->
+    { xtop, xs, ys, ytop } ~~> o ->
+    { xtop, x::xs, y::ys, ytop } ~~> o
+
+| BH_compare_head_lt : forall xtop ytop x xs y ys o,
+    length xs = length ys ->
+    xs <> [] ->
+    { x, y } ~~~> LT ->
+    check_lt_graph xs ytop o ->
+    { xtop, x::xs, y::ys, ytop } ~~> o
+
+(*
+| BH_compare_length_lt : forall x xs y ys,
+    y <> BH [] ->
+    (length xs < length ys)%nat ->
+    { x::xs, y::ys } ~~> LT
+
+| BH_compare_length_gt : forall x xs y ys,
+    x <> BH [] ->
+    (length xs > length ys)%nat ->
+    { x::xs, y::ys } ~~> GT
+
+| BH_compare_head_gt : forall x xs y ys o,
+    length xs = length ys ->
+    xs <> [] ->
+    { x, y } ~~~> GT ->
+    check_gt_graph xs (BH (y::ys)) o ->
+    { x::xs, y::ys } ~~> o
+*)
+
+where "{ a , x , y , b } ~~> z" := (BH_compare_seq_graph a x y b z)
+
+with check_lt_graph : list BHForm -> BHForm -> ordering -> Prop :=
+
+| check_lt0 : forall ytop,
+     check_lt_graph [] ytop LT
+
+| check_lt1 : forall x xs ytop o,
+     { x, ytop } ~~~> LT ->
+     check_lt_graph xs ytop o ->
+     check_lt_graph (x::xs) ytop o
+
+| check_lt2 : forall x xs ytop,
+     { x, ytop } ~~~> GT ->
+     check_lt_graph (x::xs) ytop GT
+
+(*
+with check_lt_graph : BHForm -> list BHForm -> ordering -> Prop :=
+| whatever_lt: forall x ys o, check_lt_graph x ys o
+
+with check_gt_graph : list BHForm -> BHForm -> ordering -> Prop :=
+| whatever_gt: forall xs y o, check_gt_graph xs y o
+*)
+.
+
+Scheme compare_graph_ind := Induction for BH_compare_graph Sort Prop
+ with compare_seq_graph_ind := Induction for BH_compare_seq_graph Sort Prop
+ with check_lt_ind := Induction for check_lt_graph Sort Prop.
+(*
+
+ with check_gt_ind := Induction for check_gt_graph Sort Prop.
+*)
+
+Lemma compare_graph_correct :
+  (forall (x:BHForm) (y:BHForm) (o:ordering), { x, y } ~~~> o -> ordering_correct o (BH_denote x) (BH_denote y)).
+Proof.
+  apply compare_graph_ind with
+    (P0 := fun xtop xs ys ytop o H => 
+      match xs, ys with
+      | [], [] => o = EQ
+      | [], (_::_) => o = LT
+      | (_::_), [] => o = GT
+      | (x::xtail), (y::ytail) =>
+          forall f,
+            normal_function f ->
+            BH_denote xtop ≈ BH_stack f (BH_denote x) (map BH_denote xtail) ->
+            BH_denote ytop ≈ BH_stack f (BH_denote y) (map BH_denote ytail) ->
+            ordering_correct o
+              (BH_stack f (BH_denote x) (map BH_denote xtail))
+              (BH_stack f (BH_denote y) (map BH_denote ytail))
+      end)
+    (P1 := fun xs ytop o H =>
+             match o with
+             | LT => forall x, In x xs -> BH_denote x < BH_denote ytop
+             | EQ => False
+             | GT => exists x, In x xs /\ BH_denote x > BH_denote ytop
+             end); auto.
+
+(*
+
+    (P2 := fun ys x o H => True); auto.
+*)
+
+  - intros. destruct xs; destruct ys; simpl in *; subst; simpl; auto with ord.
+    apply BH_stack_nonzero; simpl; auto with ord.
+    apply BH_stack_nonzero; simpl; auto with ord.
+  - intros. destruct o; simpl in *; auto with ord.
+    apply normal_increasing; auto with ord.
+    destruct H. split; auto with ord.
+    apply normal_increasing; auto with ord.
+  - simpl; intros. subst x.
+    destruct xs; [ congruence |].
+    destruct ys; auto.
+    intros.
+    simpl BH_denote.
+    simpl map.
+    rewrite BH_stack_leading_zero; auto with ord.
+    apply H; auto with ord.
+    rewrite H1.
+    simpl BH_denote.
+    simpl map.
+    rewrite BH_stack_leading_zero; auto with ord.
+
+  - simpl; intros. subst y.
+    destruct ys; [ congruence |].
+    destruct xs; auto.
+    intros.
+    simpl BH_denote.
+    simpl map.
+    rewrite BH_stack_leading_zero; auto with ord.
+    apply H; auto with ord.
+    rewrite H2.
+    simpl BH_denote.
+    simpl map.
+    rewrite BH_stack_leading_zero; auto with ord.
+
+  - simpl; intros.
+    destruct xs.
+    + destruct ys; subst; simpl.
+      destruct H; split; auto with ord.
+      simpl in *. congruence.
+    + destruct ys; [simpl in *; congruence |].
+      simpl in *.
+      repeat rewrite map_length in *.
+      rewrite e.
+      assert ( (BH_stack (bhtower (S (length ys)) f (BH_denote x)) 
+                  (BH_denote b1) (map BH_denote xs)) ≈
+                 (BH_stack (bhtower (S (length ys)) f (BH_denote y)) 
+                    (BH_denote b1) (map BH_denote xs))).
+      { destruct H.
+        split; apply BH_stack_monotone; auto with ord.
+        { clear; induction xs; simpl; constructor; auto with ord. }
+        { clear; induction xs; simpl; constructor; auto with ord. } }        
+      rewrite H4.
+      apply H0; auto with ord.
+      rewrite H2. rewrite e. auto with ord.
+
+  - intros. simpl in *.
+    destruct o; simpl.
+    + admit. (* maybe? non-trivial... *)
+    + contradiction.
+    + destruct H0 as [xbig [Hin Hbig]].
+      apply ord_lt_le_trans with (BH_denote xbig).
+      rewrite <- H3; auto.
+      clear -Hin H1.
+      revert x f H1.
+      induction xs; simpl; intros.
+      { elim Hin. }
+      simpl in Hin. destruct Hin; auto with ord.
+      subst a.
+      case_eq (length xs); intros.
+      * destruct xs; try (simpl in *; congruence).
+        simpl. apply normal_inflationary; auto with ord.
+      * transitivity (BH_stack
+                      (bhtower (S (length (map BH_denote xs))) f (BH_denote x))
+                      (BH_denote xbig) (stackZeros n [0])).
+        rewrite BH_stack_zeros.
+        apply (normal_inflationary (fun q => bhtower (S n)
+                                              (bhtower (S (length (map BH_denote xs))) f (BH_denote x))
+                                              q 0)); auto with ord.
+        apply BH_stack_monotone; auto with ord.
+        admit. (* very plausible *) 
+
+  - simpl; intuition.
+
+  - simpl; intros.
+    destruct o.
+    + simpl; intuition; subst; auto.
+    + assumption.
+    + destruct H0 as [q [??]].
+      exists q; simpl; intuition.
+
+  - simpl; intros.
+    exists x. simpl; intuition.
+
+Qed.
+
+
+Require Import Program.Wf.
+
+Print Acc.
+
+
+
+
+
+Ltac go := unfold BH_listSize; simpl; intros; lia.
+
+Lemma asdf1 : 
+  forall a b xs y ys,
+    (BH_termSize a + BH_termSize b <= 1 + BH_listSize xs + BH_listSize ys)%nat ->
+    (BH_termSize a + BH_termSize b <= 1 + BH_listSize xs + BH_listSize (y::ys))%nat.
+Proof.
+  unfold BH_listSize; simpl; intros; lia.
+Qed.
+
+Lemma asdf2 : 
+  forall a b x xs ys,
+    (BH_termSize a + BH_termSize b <= 1 + BH_listSize xs + BH_listSize ys)%nat ->
+    (BH_termSize a + BH_termSize b <= 1 + BH_listSize (x::xs) + BH_listSize ys)%nat.
+Proof.
+  unfold BH_listSize; simpl; intros; lia.
+Qed.
+
+Lemma asdf3 :
+  forall a b x xs y ys,
+    (BH_termSize a + BH_termSize b <= 1 + BH_listSize xs + BH_listSize ys)%nat ->
+    (BH_termSize a + BH_termSize b <= 1 + BH_listSize (x::xs) + BH_listSize (y::ys))%nat.
+Proof.
+  unfold BH_listSize; simpl; intros; lia.
+Qed.
+
+
+Fixpoint BH_compare_seq
+  (xs:list BHForm) :
+  forall (ys:list BHForm),
+  (forall a b (H:(BH_termSize a + BH_termSize b <= 1 + BH_listSize xs + BH_listSize ys)%nat), ordering) -> ordering :=
+  
+    match xs as xs' return
+          forall ys, 
+            (forall a b (H:(BH_termSize a + BH_termSize b <= 1 + BH_listSize xs' + BH_listSize ys)%nat), ordering) -> ordering with
+    | [] =>
+        fun ys => match ys with
+                  | [] => fun _ => EQ
+                  | (_::_) => fun _ => LT
+                  end
+    | x::xtail =>
+        fix inner (ys:list BHForm) : 
+        (forall a b (H:(BH_termSize a + BH_termSize b <= 1 + BH_listSize (x::xtail) + BH_listSize ys)%nat), ordering) -> ordering :=
+
+          match ys as ys' return 
+                (forall a b (H:(BH_termSize a + BH_termSize b <= 1 + BH_listSize (x::xtail) + BH_listSize ys')%nat), ordering) -> ordering with
+          | []  => fun _ => GT
+          | (y::ytail) =>
+              fun rec =>
+              if isNil xtail then
+                if isNil ytail then rec x y ltac:(go) else
+                   if bh_isZero y then (inner ytail (fun a b H => rec a b (asdf1 a b (x::xtail) y ytail H)))
+                  else LT
+              else
+                if bh_isZero x then BH_compare_seq xtail (y::ytail) (fun a b H => rec a b (asdf2 a b x xtail (y::ytail) H)) else
+                  if isNil ytail then GT else
+                    if bh_isZero y then (inner ytail (fun a b H => rec a b (asdf1 a b (x::xtail) y ytail H))) else
+                      (* x is nonzero, y is nonzero, xs is nonnil, ys is nonnil *)
+                      match nat_compare (length xtail) (length ytail) with
+                      | LT => LT
+                      | EQ => match rec x y ltac:(go) with
+                              | LT => LT
+                              | EQ => BH_compare_seq xtail ytail (fun a b H => rec a b (asdf3 a b x xtail y ytail H))
+                              | GT => GT
+                              end
+                      | GT => GT
+                      end
+          end
+    end.
+
+
+Lemma asdf0 : forall a b xs ys,
+ (BH_termSize a + BH_termSize b <= 1 + BH_listSize xs + BH_listSize ys)%nat ->
+ (BH_termSize a + BH_termSize b < BH_termSize (BH xs) + BH_termSize (BH ys))%nat.
+Proof.
+  unfold BH_listSize.
+  simpl; intros. 
+  lia.
+Qed.
+
+Definition BH_compare_def
+  (x:BHForm) (y:BHForm) :
+  (forall a b (H:(BH_termSize a + BH_termSize b < BH_termSize x + BH_termSize y)%nat), ordering) -> ordering :=
+
+  match x as x', y as y' return 
+        (forall a b (H:(BH_termSize a + BH_termSize b < BH_termSize x' + BH_termSize y')%nat), ordering) -> ordering with
+  | BH xs, BH ys =>
+      fun rec => BH_compare_seq xs ys (fun a b H => rec a b (asdf0 a b xs ys H))
+  end.
+
+
+Fixpoint BH_compare_WF (x:BHForm) (y:BHForm)
+  (WF:Acc lt (BH_termSize x + BH_termSize y)%nat) {struct WF} : ordering :=
+
+  match WF with
+  | Acc_intro _ WF' => BH_compare_def x y (fun x' y' H => BH_compare_WF x' y' (WF' _ H))
+  end.
+
+Definition BH_compare (x:BHForm) (y:BHForm) : ordering :=
+  BH_compare_WF x y (Wf_nat _).
+
+
+
+Fixpoint BH_compare (x:BHForm) : BHForm -> ordering :=
+  fix inner (y:BHForm) : ordering :=
+    match x, y with
+    | BH xs0, BH ys0 =>
+        (fix compare_sequence (xs:list BHForm) : list BHForm -> ordering :=
+           fix compare_sequence_inner (ys:list BHForm) : ordering :=
+             match xs with
+             | []  => if bh_isZero y then EQ else LT
+             | [x] =>  match ys with
+                       | []  => GT
+                       | [y] => BH_compare x y
+                       | _   => LT
+                       end
+             | (x::xs) =>
+                 if bh_isZero x then compare_sequence xs ys else
+                   match ys with
+                   | []  => GT
+                   | (y::ytail) =>
+                       if isNil ytail then LT else
+                         if bh_isZero y then compare_sequence_inner ytail else
+                           match nat_compare (length xs) (length ytail) with
+                           | LT => LT
+                           | EQ => match BH_compare x y with
+                                   | LT => (fix check_lt (xs:list BHForm) :=
+                                              match xs with
+                                              | [] => LT
+                                              | (x'::xs') =>
+                                                  match BH_compare x' y with
+                                                  | LT => check_lt xs'
+                                                  | EQ => if bh_allZero (x'::xs') then EQ else GT
+                                                  | GT => GT
+                                                  end
+                                              end
+                                           ) xs
+                                   | EQ => compare_sequence xs ytail
+                                   | GT => (fix check_gt (ys':list BHForm) :=
+                                              match ys' with
+                                              | [] => GT
+                                              | (y'::ys'') =>
+                                                  match inner y' with
+                                                  | LT => LT
+                                                  | EQ => if bh_allZero ys' then EQ else LT
+                                                  | GT => check_gt ys''
+                                                  end
+                                              end
+                                           ) ytail
+                                   end
+                           | GT => GT
+                           end
+                   end
+             end) xs0 ys0
+    end. 
